Validator/Learning/ImperativeBasic.lean
@@ -16,47 +16,39 @@ import Validator.Learning.ImperativeLeave
 namespace ImperativeBasic
 
 -- foldLoop is a more readable version of List.foldlM for imperative programmers:
-private def foldLoop (deriv: Rules μ α Pred -> Hedge.Node α -> Except String (Rules μ α Pred)) (start: Rules μ α Pred) (hedge: Hedge α): Except String (Rules μ α Pred) := do
+private def foldLoop (deriv: List (Rule μ α Pred) -> Hedge.Node α -> List (Rule μ α Pred)) (start: List (Rule μ α Pred)) (hedge: Hedge α): Id (List (Rule μ α Pred)) := do
   let mut res := start
   for tree in hedge do
-    match deriv res tree with
-    | Except.error err => throw err
-    | Except.ok r => res := r
+    res := deriv res tree
   return res
 
-def derive [DecidableEq α] (g: Grammar μ α Pred) (xs: Rules μ α Pred) (tree: Hedge.Node α): Except String (Rules μ α Pred) :=
+def derive [DecidableEq α] (g: Grammar μ α Pred) (xs: List (Rule μ α Pred)) (tree: Hedge.Node α): List (Rule μ α Pred) :=
   -- If all expressions are unescapable, then simply return without look at the input tree.
   -- An example of an unescapable expression is emptyset, since its derivative is always emptyset, no matter the input.
   if List.all xs Regex.unescapable
-  then Except.ok xs
+  then xs
   else
     -- Desconstruct the tree to retrieve its label and children
     match tree with
     | Hedge.Node.mk label children =>
       -- enters is one of our two new memoizable functions.
-      let ifexprs: IfExprs μ α := Enter.deriveEnter xs
+      let ifexprs: List (IfExpr μ α) := Enter.deriveEnter_list xs
       -- childxs = expressions to evaluate on children.
-      let childxs: Rules μ α Pred := IfExpr.evals g ifexprs label
+      let childxs: List (Rule μ α Pred) := List.map (fun x => IfExpr.eval g x label) ifexprs
       -- dchildxs = derivatives of children. The ' is for the exception it is wrapped in.
       -- see foldLoop for an explanation of what List.foldM does.
-      let dchildxs': Except String (Rules μ α Pred) := List.foldlM (derive g) childxs children
-      match dchildxs' with
-      | Except.error err => Except.error err
-      | Except.ok dchildxs =>
+      let dchildxs: List (Rule μ α Pred) := List.foldl (derive g) childxs children
       -- dxs = derivatives of xs. The ' is for the exception it is wrapped in.
       -- leaves is the other one of our two new memoizable functions.
-      let dxs': Except String (Rules μ α Pred) := ImperativeLeave.deriveLeave xs (List.map Regex.nullable dchildxs)
-      match dxs' with
-      | Except.error err => Except.error err
-      | Except.ok dxs => Except.ok dxs
+      let dxs: List (Rule μ α Pred) := ImperativeLeave.deriveLeave xs (List.map Regex.nullable dchildxs)
+      dxs
 
 def derivs [DecidableEq α] (g: Grammar μ α Pred) (x: Rule μ α Pred) (hedge: Hedge α): Except String (Rule μ α Pred) :=
   -- see foldLoop for an explanation of what List.foldM does.
-  let dxs := List.foldlM (derive g) [x] hedge
+  let dxs := List.foldl (derive g) [x] hedge
   match dxs with
-  | Except.error err => Except.error err
-  | Except.ok [dx] => Except.ok dx
-  | Except.ok _ => Except.error "expected one expression"
+  | [dx] => Except.ok dx
+  | _ => Except.error "expected one expression"
 
 def validate [DecidableEq α] (g: Grammar μ α Pred) (x: Rule μ α Pred) (hedge: Hedge α): Except String Bool :=
   match derivs g x hedge with
