Validator/Learning/ImperativeCompress.lean
@@ -18,36 +18,100 @@ import Validator.Learning.ImperativeLeave
 
 namespace ImperativeCompress
 
+inductive Index where
+ | val (n: Nat)
+ | emptyset
+
+def indexOf [DecidableEq α] (xs: List (Regex (Pred α × Ref μ))) (y: (Rule μ α Pred)): Except String Index :=
+  match y with
+  | Regex.emptyset => Except.ok Index.emptyset
+  | _ =>
+    match List.idxOf? y xs with
+    | Option.none => Except.error "indexOf: unable to find expression"
+    | Option.some idx => Except.ok (Index.val idx)
+
+def ofIndex' (xs: List (Rule μ α Pred)) (index: Nat): Except String (Rule μ α Pred) :=
+  match xs with
+  | [] => Except.error "index overflow"
+  | x::xs' =>
+    match index with
+    | 0 => Except.ok x
+    | (n' + 1) => ofIndex' xs' n'
+
+def ofIndex (xs: List (Rule μ α Pred)) (index: Index): Except String (Rule μ α Pred) :=
+  match index with
+  | Index.emptyset => Except.ok Regex.emptyset
+  | Index.val n =>
+    ofIndex' xs n
+
+-- Indices represents compressed indexes
+-- that resulted from compressing a list of expressions.
+-- This can be used to expanded to a list of expressions.
+inductive Indices where
+  | mk (indices: List Index)
+
+def compressed [DecidableEq α] (xs: Rules μ α Pred ν): Nat :=
+  (List.erase (List.eraseReps xs.toList) Regex.emptyset).length
+
+-- compress compresses a list of expressions.
+def compress [DecidableEq α] (xs: List (Rule μ α Pred)): Except String ((List (Rule μ α Pred)) × Indices) := do
+  -- sort to increase chance of cache hit
+  -- TODO: let sxs := List.mergeSort xs
+
+  -- remove duplicates
+  let sxs' := List.eraseReps xs
+
+  -- remove unescapable expressions, currently only emptyset
+  let sxs'' := List.erase sxs' Regex.emptyset
+
+  -- find all indexes of the original expressions in the compressed expressions
+  let indexes: List Index <- List.mapM (indexOf sxs'') xs
+  return (
+    Subtype.mk
+      sxs'' (by
+        simp only [sxs'', sxs']
+        rfl
+      ),
+    Indices.mk indexes
+  )
+
+-- expand expands a list of expressions.
+def expand (indices: Indices) (xs: List (Rule μ α Pred)): Except String (List (Rule μ α Pred)) :=
+  match indices with
+  | Indices.mk indexes =>
+    match MonadExcept.ofExcept (List.mapM (ofIndex xs) indexes) with
+    | Except.error e => Except.error e
+    | Except.ok k => Except.ok k
+
 -- deriv is the same as ImperativeBasic's deriv function, except that it includes the use of the compress and expand functions.
-def derive [DecidableEq α] (g: Grammar μ α Pred) (xs: Rules μ α Pred) (t: Hedge.Node α): Except String (Rules μ α Pred) :=
+def derive [DecidableEq α] (g: Grammar μ α Pred) (xs: List (Rule μ α Pred)) (t: Hedge.Node α): Except String (List (Rule μ α Pred)) :=
   if List.all xs Regex.unescapable
   then Except.ok xs
   else
     match t with
     | Hedge.Node.mk label children =>
-      let ifexprs: IfExprs μ α := Enter.deriveEnter xs
-      let childxs: Rules μ α Pred := IfExpr.evals g ifexprs label
+      let ifexprs: List (IfExpr μ α) := Enter.deriveEnter_list xs
+      -- List.Vector.map (fun x => eval g x t) ifExprs
+      let childxs: List (Rule μ α Pred) := List.map (fun x => IfExpr.eval g x label) ifexprs
       -- cchildxs' = compressed expressions to evaluate on children. The ' is for the exception it is wrapped in.
-      let cchildxs' : Except String ((Rules μ α Pred) × Compress.Indices) := Compress.compress childxs
+      let cchildxs' : Except String ((List (Rule μ α Pred)) × Indices) := compress childxs
       match cchildxs' with
       | Except.error err => Except.error err
       | Except.ok (cchildxs, indices) =>
       -- cdchildxs = compressed derivatives of children. The ' is for the exception it is wrapped in.
       -- see foldLoop for an explanation of what List.foldM does.
-      let cdchildxs' : Except String (Rules μ α Pred) := List.foldlM (derive g) cchildxs children
+      let cdchildxs' : Except String (List (Rule μ α Pred)) := List.foldlM (derive g) cchildxs children
       match cdchildxs' with
       | Except.error err => Except.error err
       | Except.ok cdchildxs =>
       -- dchildxs = uncompressed derivatives of children. The ' is for the exception it is wrapped in.
-      let dchildxs' := Compress.expand indices cdchildxs
+      let dchildxs' := expand indices cdchildxs
       match dchildxs' with
       | Except.error err => Except.error err
       | Except.ok dchildxs =>
       -- dxs = derivatives of xs. The ' is for the exception it is wrapped in.
-      let dxs': Except String (Rules μ α Pred) := ImperativeLeave.deriveLeave xs (List.map Rule.nullable dchildxs)
-      match dxs' with
-      | Except.error err => Except.error err
-      | Except.ok dxs => Except.ok dxs
+      let dxs: List (Rule μ α Pred) := ImperativeLeave.deriveLeave xs (List.map Rule.nullable dchildxs)
+      Except.ok dxs
 
 def derivs [DecidableEq α] (g: Grammar μ α Pred) (x: Rule μ α Pred) (hedge: Hedge α): Except String (Rule μ α Pred) :=
   -- see foldLoop for an explanation of what List.foldM does.
