Validator/Learning/ImperativeLeave.lean
@@ -6,63 +6,44 @@ import Validator.Expr.Regex
 
 namespace ImperativeLeave
 
-def leave (x: Rule μ α Pred) (ns: List Bool): Except String (Rule μ α Pred × List Bool) :=
+def leave (x: Rule μ α Pred) (ns: List Bool): (Rule μ α Pred × List Bool) :=
   match x with
-  | Regex.emptyset => Except.ok (Regex.emptyset, ns)
-  | Regex.emptystr => Except.ok (Regex.emptyset, ns)
+  | Regex.emptyset => (Regex.emptyset, ns)
+  | Regex.emptystr => (Regex.emptyset, ns)
   | Regex.symbol _ =>
     match ns with
-    | [] => Except.error "wtf"
+    | [] =>
+      -- impossible and handled properly with a Vector in non-imperative/proper implementations.
+      (x, ns)
     | (null::ns') =>
       if null
-      then Except.ok (Regex.emptystr, ns')
-      else Except.ok (Regex.emptyset, ns')
+      then (Regex.emptystr, ns')
+      else (Regex.emptyset, ns')
   | Regex.or y z =>
-    match leave y ns with
-    | Except.error e => Except.error e
-    | Except.ok (y', ns') =>
-      match leave z ns' with
-      | Except.error e => Except.error e
-      | Except.ok (z', ns'') =>
-        Except.ok (Regex.or y' z', ns'')
+    let (y', ns') := leave y ns
+    let (z', ns'') := leave z ns'
+    (Regex.or y' z', ns'')
   | Regex.concat y z =>
     if Regex.nullable y
     then
-      match leave y ns with
-      | Except.error e => Except.error e
-      | Except.ok (y', ns') =>
-        match leave z ns' with
-        | Except.error e => Except.error e
-        | Except.ok (z', ns'') =>
-          Except.ok (Regex.or (Regex.concat y' z) z', ns'')
+      let (y', ns') := leave y ns
+      let (z', ns'') := leave z ns'
+      (Regex.or (Regex.concat y' z) z', ns'')
     else
-      match leave y ns with
-      | Except.error e => Except.error e
-      | Except.ok (y', ns') =>
-        Except.ok (Regex.concat y' z, ns')
+      let (y', ns') := leave y ns
+      (Regex.concat y' z, ns')
   | Regex.star y =>
-      match leave y ns with
-      | Except.error e => Except.error e
-      | Except.ok (y', ns') =>
-        Except.ok (Regex.star y', ns')
+      let (y', ns') := leave y ns
+      (Regex.star y', ns')
 
 -- deriveLeave takes a list of expressions and list of bools.
 -- The list of bools represent the nullability of the derived child expressions.
 -- Each bool will then replace each tree expression with either an epsilon or emptyset.
 -- The lists do not to be the same length, because each expression can contain an arbitrary number of tree expressions.
-def deriveLeave (xs: Rules μ α Pred) (ns: List Bool): Except String (Rules μ α Pred) :=
+def deriveLeave (xs: List (Rule μ α Pred)) (ns: List Bool): List (Rule μ α Pred) :=
   match xs with
-  | [] =>
-    match ns with
-    | [] => Except.ok []
-    | _ => Except.error "Not all nulls were consumed, but there are no expressions to place them in."
+  | [] => []
   | (x::xs') =>
-    let lx': Except String (Rule μ α Pred × List Bool) := leave x ns
-    match lx' with
-    | Except.error err => Except.error err
-    | Except.ok (lx, tailns) =>
-    let lxs': Except String (Rules μ α Pred) := deriveLeave xs' tailns
-    match lxs' with
-    | Except.error err => Except.error err
-    | Except.ok lxs =>
-      Except.ok (lx::lxs)
+    let (lx, tailns): (Rule μ α Pred × List Bool) := leave x ns
+    let lxs: List (Rule μ α Pred) := deriveLeave xs' tailns
+    lx::lxs
