Validator/Learning/Parser.lean
@@ -20,22 +20,22 @@ import Validator.Validator.Inst.TreeParserM
 
 namespace Parser
 
-def deriveEnter [DecidableEq α] [ValidateM m μ α] (g: Grammar μ α Pred) (xs: Rules μ α Pred): m (Rules μ α Pred) := do
+def deriveEnter [DecidableEq α] [ValidateM m μ α ν] (g: Grammar μ α Pred) (xs: Rules μ α Pred ν): m (Rules μ α Pred (Symbol.nums xs)) := do
   let enters <- Enter.DeriveEnter.deriveEnter xs
   let token <- Parser.token
   return IfExpr.evals g enters token
 
-def deriveLeaveM [DecidableEq α] [ValidateM m μ α] (xs: Rules μ α Pred) (cs: Rules μ α Pred): m (Rules μ α Pred) :=
-  Leave.DeriveLeaveM.deriveLeaveM xs (List.map Rule.nullable cs)
+def deriveLeaveM [DecidableEq α] [ValidateM m μ α ν] (xs: Rules μ α Pred ν) (cs: Rules μ α Pred (Symbol.nums xs)): m (Rules μ α Pred ν) :=
+  Leave.DeriveLeaveM.deriveLeaveM xs (List.Vector.map Rule.nullable cs)
 
-def deriveValue [DecidableEq α] [ValidateM m μ α] (g: Grammar μ α Pred) (xs: Rules μ α Pred): m (Rules μ α Pred) := do
+def deriveValue [DecidableEq α] [ValidateM m μ α ν] (g: Grammar μ α Pred) (xs: Rules μ α Pred ν): m (Rules μ α Pred ν) := do
   deriveEnter g xs >>= deriveLeaveM xs
 
 -- TODO: Is it possible to have a Parser type that can be proved to be of the correct shape, and have not expection throwing
 -- for example: can you prove that your Parser will never return an Hint.leave after returning a Hint.field.
 -- This class can be called the LawfulParser.
-partial def derive [DecidableEq α] [ValidateM m μ α] (g: Grammar μ α Pred) (xs: Rules μ α Pred): m (Rules μ α Pred) := do
-  if List.all xs Regex.unescapable then
+partial def derive [DecidableEq α] [ValidateM m μ α ν] (g: Grammar μ α Pred) (xs: Rules μ α Pred ν): m (Rules μ α Pred ν) := do
+  if List.all xs.toList Regex.unescapable then
     Parser.skip; return xs
   match <- Parser.next with
   | Hint.field =>
@@ -52,11 +52,9 @@ partial def derive [DecidableEq α] [ValidateM m μ α] (g: Grammar μ α Pred) 
   | Hint.leave => return xs -- never happens at the top
   | Hint.eof => return xs -- only happens at the top
 
-def validate {m} [DecidableEq α] [ValidateM m μ α] (g: Grammar μ α Pred) (x: Rule μ α Pred): m Bool := do
-  let dxs <- derive g [x]
-  match dxs with
-  | [dx] => return Rule.nullable dx
-  | _ => throw "expected one expression"
+def validate {m} [DecidableEq α] [ValidateM m μ α ν] (g: Grammar μ α Pred) (x: Rule μ α Pred): m Bool := do
+  let dxs <- derive g (List.Vector.cons x List.Vector.nil)
+  return Rule.nullable dxs.head
 
 def run [DecidableEq α] (g: Grammar μ α Pred) (t: Hedge.Node α): Except String Bool :=
   TreeParserM.run' (validate g g.start) t
