Validator/Std/Vec.lean
@@ -1,0 +1,7 @@
+import Mathlib.Data.Vector.Basic
+import Mathlib.Data.Vector.Snoc
+
+namespace Vec
+
+def fromList (xs: List α): List.Vector α (xs.length) :=
+  Subtype.mk xs rfl
